src/Prototype/Reduction.v
@@ -2,75 +2,57 @@ Require Import List String Peano_dec.
 Require Import FnMap Language.
 
 Section Reduction.
-  (* Variable MsgT StateT: Type. *)
+  Variable MsgT StateT: Type.
 
-  (* Local Notation MsgId := (MsgId MsgT). *)
+  Local Notation MsgId := (MsgId MsgT).
+  Local Notation Label := (Label MsgT).
 
-  (* Definition Reduced (from to: list MsgId) (msg1 msg2: MsgId) := *)
-  (*   exists hst1 hst2, *)
-  (*     from = hst1 ++ msg1 :: msg2 :: hst2 /\ *)
-  (*     to = hst1 ++ msg2 :: msg1 :: hst2. *)
+  Definition Reduced (from to: list Label) (lbl1 lbl2: Label) :=
+    exists hst1 hst2,
+      from = hst1 ++ lbl1 :: lbl2 :: hst2 /\
+      to = hst1 ++ lbl2 :: lbl1 :: hst2.
 
-  (* Lemma reduction_preserves_steps': *)
-  (*   forall {StateT} (msg1 msg2: MsgId), *)
-  (*     (* msgFrom (msgOf msg1) <> msgFrom (msgOf msg2) -> *) *)
-  (*     forall (obs: Objects MsgT StateT) oss1 oims1 oss2 oims2 hst2 hst1, *)
-  (*       steps obs oss1 oims1 (hst1 ++ msg1 :: msg2 :: hst2) oss2 oims2 -> *)
-  (*       steps obs oss1 oims1 (hst1 ++ msg2 :: msg1 :: hst2) oss2 oims2. *)
-  (* Admitted. *)
+  Lemma reduction_preserves_steps'':
+    forall {StateT} (lbl1 lbl2: Label),
+      msgTo (lbl_in lbl1) <> msgFrom (lbl_in lbl2) ->
+      msgTo (lbl_in lbl1) <> msgTo (lbl_in lbl2) ->
+      forall (obs: Objects MsgT StateT) oss1 oims1 oss2 oims2 hst,
+        steps obs oss1 oims1 (lbl1 :: lbl2 :: hst) oss2 oims2 ->
+        steps obs oss1 oims1 (lbl2 :: lbl1 :: hst) oss2 oims2.
+  Proof.
+    intros.
+    inversion_clear H1; inversion_clear H2.
 
-  (* Theorem reduction_preserves_steps: *)
-  (*   forall obs oss1 oims1 hst oss2 oims2, *)
-  (*     steps obs oss1 oims1 hst oss2 oims2 -> *)
-  (*     forall msg1 msg2 hst', *)
-  (*       Reduced hst hst' msg1 msg2 -> *)
-  (*       (* Different sources ->  *) *)
-  (* (*        * Messages were handled by different objects ->  *) *)
-  (* (*        * Disjoint state transitions! *) *)
-  (* (*        *) *)
-  (*       msgFrom (msgOf msg1) <> msgFrom (msgOf msg2) -> *)
-  (*       steps obs oss1 oims1 hst' oss2 oims2. *)
-  (* Proof. *)
-  (*   unfold Reduced; intros. *)
-  (*   destruct H0 as [hst1 [hst2 [? ?]]]; subst. *)
-  (*   apply reduction_preserves_steps'; auto. *)
-  (* Qed. *)
+    repeat econstructor; try eassumption; clear H1.
+  Admitted.
+  
+  Lemma reduction_preserves_steps':
+    forall {StateT} (lbl1 lbl2: Label),
+      msgTo (lbl_in lbl1) <> msgFrom (lbl_in lbl2) ->
+      msgTo (lbl_in lbl1) <> msgTo (lbl_in lbl2) ->
+      forall (obs: Objects MsgT StateT) hst1 oss1 oims1 oss2 oims2 hst2,
+        steps obs oss1 oims1 (hst1 ++ lbl1 :: lbl2 :: hst2) oss2 oims2 ->
+        steps obs oss1 oims1 (hst1 ++ lbl2 :: lbl1 :: hst2) oss2 oims2.
+  Proof.
+    induction hst1; simpl; intros.
+    - apply reduction_preserves_steps''; auto.
+    - inversion_clear H1.
+      econstructor; eauto.
+  Qed.
 
-  (* Definition ReducedM (from to msgs: list Msg) (tmsg: Msg) := *)
-  (*   exists hst1 hst2, *)
-  (*     from = hst1 ++ msgs ++ tmsg :: hst2 /\ *)
-  (*     to = hst1 ++ tmsg :: msgs ++ hst2. *)
-
-  (* Lemma reductions_preserve_steps': *)
-  (*   forall (tmsg: Msg) msgs, *)
-  (*     Forall (fun m => msg_from m <> msg_from tmsg) msgs -> *)
-  (*     forall obs oss1 oims1 oss2 oims2 hst2 hst1, *)
-  (*       steps obs oss1 oims1 (hst1 ++ msgs ++ tmsg :: hst2) oss2 oims2 -> *)
-  (*       steps obs oss1 oims1 (hst1 ++ tmsg :: msgs ++ hst2) oss2 oims2. *)
-  (* Proof. *)
-  (*   induction msgs; simpl; intros; auto. *)
-
-  (*   replace (hst1 ++ a :: msgs ++ tmsg :: hst2) *)
-  (*   with ((hst1 ++ a :: nil) ++ msgs ++ tmsg :: hst2) in H0 *)
-  (*     by (repeat rewrite <-app_assoc; reflexivity). *)
-  (*   inversion_clear H; apply IHmsgs in H0; auto. *)
-
-  (*   rewrite <-app_assoc in H0; simpl in H0. *)
-  (*   apply reduction_preserves_steps'; auto. *)
-  (* Qed. *)
-
-  (* Theorem reductions_preserve_steps: *)
-  (*   forall obs oss1 oims1 hst oss2 oims2, *)
-  (*     steps obs oss1 oims1 hst oss2 oims2 -> *)
-  (*     forall msgs tmsg hst', *)
-  (*       ReducedM hst hst' msgs tmsg -> *)
-  (*       Forall (fun m => msg_from m <> msg_from tmsg) msgs -> *)
-  (*       steps obs oss1 oims1 hst' oss2 oims2. *)
-  (* Proof. *)
-  (*   unfold ReducedM; intros. *)
-  (*   destruct H0 as [hst1 [hst2 [? ?]]]; subst. *)
-  (*   apply reductions_preserve_steps'; auto. *)
-  (* Qed. *)
+  Theorem reduction_preserves_steps:
+    forall (obs: Objects MsgT StateT) oss1 oims1 hst oss2 oims2,
+      steps obs oss1 oims1 hst oss2 oims2 ->
+      forall lbl1 lbl2 hst',
+        Reduced hst hst' lbl1 lbl2 ->
+        msgTo (lbl_in lbl1) <> msgFrom (lbl_in lbl2) ->
+        msgTo (lbl_in lbl1) <> msgTo (lbl_in lbl2) ->
+        steps obs oss1 oims1 hst' oss2 oims2.
+  Proof.
+    unfold Reduced; intros.
+    destruct H0 as [hst1 [hst2 [? ?]]]; subst.
+    apply reduction_preserves_steps'; auto.
+  Qed.
 
 End Reduction.
         
